PAC_Checker_LLVM/IICF_HashMap.thy
@@ -1,0 +1,907 @@
+theory IICF_HashMap
+  imports IICF_PartialMap IICF_HashSet Isabelle_LLVM.Proto_EOArray
+begin
+
+text \<open>Hashmap implementation, based on the existing {IICF_PartialMap} and the Hashable interface.
+  We reuse the bucket implementation from {IICF_HashSet}.\<close>
+
+text \<open>TODO list \<emdash> coverage of the @{theory Isabelle_LLVM.IICF_Map} interface
+  \<^item> [x] \<open>op_map_empty\<close> (\<open>lshm_empty\<close>, parametric in the initial number of buckets)
+  \<^item> [x] \<open>op_map_update\<close>
+  \<^item> [x] \<open>op_map_delete\<close>
+  \<^item> [x] \<open>op_map_contains_key\<close>
+  \<^item> [ ] \<open>op_map_is_empty\<close> - Expensive without length in cl_list...
+  \<^item> [x] \<open>op_map_lookup\<close>
+  \<^item> [ ] \<open>op_map_the_lookup\<close>
+
+  Infrastructure (not interface ops):
+  \<^item> [x] \<open>MK_FREE\<close> bucket entry free (\<open>bucket_free_rule\<close>)
+  \<^item> [ ] \<open>MK_FREE\<close> deep free of the whole map
+\<close>
+
+type_synonym ('k, 'v) hashmap = \<open>('k \<times> 'v) list list\<close>
+
+locale hashmap_env =
+  key: freeable_assn K kfree +
+  val: copyable_assn V vfree vcopy +
+  eq_assn K keq + hashable_assn K khash khash_impl
+  for K :: \<open>'k \<Rightarrow> 'ki::llvm_rep \<Rightarrow> assn\<close>
+  and kfree :: \<open>'ki \<Rightarrow> unit llM\<close>
+  and V :: \<open>'v \<Rightarrow> 'vi::llvm_rep \<Rightarrow> assn\<close>
+  and vfree :: \<open>'vi \<Rightarrow> unit llM\<close>
+  and vcopy :: \<open>'vi \<Rightarrow> 'vi llM\<close>
+  and keq :: \<open>'ki \<Rightarrow> 'ki \<Rightarrow> 1 word llM\<close>
+  and khash :: \<open>'k \<Rightarrow> 64 word\<close>
+  and khash_impl :: \<open>'ki \<Rightarrow> 64 word llM\<close>
+begin
+
+definition vopt_assn :: \<open>'v option \<Rightarrow> 'vi ptr \<Rightarrow> assn\<close> where
+  \<open>vopt_assn w p \<equiv> case w of None \<Rightarrow> \<up>(p = null) | Some v \<Rightarrow> \<upharpoonleft>(box_assn V) v p\<close>
+
+lemma vopt_assn_simps[simp]:
+  \<open>vopt_assn None p = \<up>(p = null)\<close>
+  \<open>vopt_assn (Some v) p = \<upharpoonleft>(box_assn V) v p\<close>
+  unfolding vopt_assn_def by simp_all
+
+text \<open>A bucket entry keeps the key inline in the node \<emdash> probing needs no indirection \<emdash>
+  and boxes only the value.\<close>
+abbreviation \<open>boxed_bucket_assn \<equiv> K \<times>\<^sub>a (\<lambda>v. vopt_assn (Some v))\<close>
+abbreviation \<open>boxed_buckets_assn \<equiv> cl_assn' boxed_bucket_assn\<close>
+
+definition bucket_free where [llvm_code, llvm_inline]:
+  \<open>bucket_free \<equiv> \<lambda>(ki,bv). doM {kfree ki; box_free vfree bv}\<close>
+
+lemma bucket_free_rule[sepref_frame_free_rules]: \<open>MK_FREE boxed_bucket_assn bucket_free\<close>
+  supply [vcg_rules] = MK_FREED[OF box_free_rule[OF val.afree_free]]
+  unfolding bucket_free_def
+  apply (rule MK_FREEI)
+  by vcg
+
+interpretation bucket: freeable_assn boxed_bucket_assn bucket_free
+  by unfold_locales (rule bucket_free_rule)
+
+term bucket.cl_free
+
+section \<open>High-level Hashmap by nested lists.\<close>
+text \<open>Like in IICF_Partial_Map, we first use abstract nested lists which we then refine down
+  to llM level.\<close>
+
+definition \<open>lshm_bucket_of n k \<equiv> unat (khash k) mod n\<close>
+definition lshm_invar :: \<open>('k, 'v) hashmap \<Rightarrow> bool\<close> where
+  \<open>lshm_invar xs \<equiv> xs\<noteq>[] \<and> (\<forall>i < length xs.
+  (distinct (map fst (xs!i))) \<and> (\<forall>(k,v) \<in> set (xs!i). lshm_bucket_of (length xs) k = i))\<close>
+definition lshm_\<alpha> :: \<open>('k, 'v) hashmap \<Rightarrow> 'k \<Rightarrow> 'v option\<close> where
+  \<open>lshm_\<alpha> xs k \<equiv> map_of (xs ! lshm_bucket_of (length xs) k) k\<close>
+definition \<open>lshm_rel \<equiv> br lshm_\<alpha> lshm_invar\<close>
+
+subsection \<open>High Level Implementation\<close>
+
+definition \<open>lshm_op_map_empty n \<equiv> replicate n ([] :: ('k \<times> 'v) list)\<close>
+
+term op_map_update
+fun lshm_bucket_update :: \<open>'k \<Rightarrow> 'v \<Rightarrow> ('k \<times> 'v) list \<Rightarrow> ('k \<times> 'v) list\<close> where
+  \<open>lshm_bucket_update k v [] = [(k, v)]\<close>
+| \<open>lshm_bucket_update k v ((kc, vc) # xs) =
+  (if k = kc then (k, v) # xs else (kc, vc) # lshm_bucket_update k v xs)\<close> 
+definition \<open>lshm_op_map_update k v xs \<equiv>
+  let bi = lshm_bucket_of (length xs) k in xs[bi:=lshm_bucket_update k v (xs!bi)]\<close>
+
+term op_map_delete
+fun lshm_bucket_delete :: \<open>'k \<Rightarrow> ('k \<times> 'v) list \<Rightarrow> ('k \<times> 'v) list\<close> where
+  \<open>lshm_bucket_delete _ [] = []\<close>
+| \<open>lshm_bucket_delete k ((ki, vi) # xs) =
+  (if k = ki then xs else (ki, vi) # lshm_bucket_delete k xs)\<close>
+definition \<open>lshm_op_map_delete k xs \<equiv>
+  let bi = lshm_bucket_of (length xs) k in xs[bi:=lshm_bucket_delete k (xs!bi)]\<close>
+
+fun lshm_bucket_contains :: \<open>'k \<Rightarrow> ('k \<times> 'v) list \<Rightarrow> bool\<close> where
+  \<open>lshm_bucket_contains _ [] = False\<close>
+| \<open>lshm_bucket_contains k ((ki, _) # xs) = (if k = ki then True else lshm_bucket_contains k xs)\<close>
+definition \<open>lshm_op_map_contains_key k xs \<equiv>
+  let bi = lshm_bucket_of (length xs) k in lshm_bucket_contains k (xs!bi)\<close>
+
+fun lshm_bucket_lookup :: \<open>'k \<Rightarrow> ('k \<times> 'v) list \<Rightarrow> 'v option\<close> where
+  \<open>lshm_bucket_lookup _ [] = None\<close>
+| \<open>lshm_bucket_lookup k ((ki, vi) # xs) = (if k = ki then Some vi else lshm_bucket_lookup k xs)\<close>
+definition \<open>lshm_op_map_lookup k xs \<equiv>
+  let bi = lshm_bucket_of (length xs) k in lshm_bucket_lookup k (xs!bi)\<close>
+
+term op_map_the_lookup
+fun lshm_bucket_the_lookup :: \<open>'k \<Rightarrow> ('k \<times> 'v) list \<Rightarrow> 'v\<close> where
+  \<open>lshm_bucket_the_lookup _ [] = undefined\<close>
+| \<open>lshm_bucket_the_lookup k ((ki, vi) # xs) = (if k = ki then vi else lshm_bucket_the_lookup k xs)\<close>
+definition \<open>lshm_the_lookup k xs \<equiv>
+  let bi = lshm_bucket_of (length xs) k in lshm_bucket_the_lookup k (xs!bi)\<close>
+
+lemma lshm_empty_fref:
+  assumes \<open>0 < n\<close>
+  shows \<open>(lshm_op_map_empty n, op_map_empty) \<in> lshm_rel\<close>
+  unfolding lshm_rel_def lshm_\<alpha>_def lshm_bucket_of_def in_br_conv
+    lshm_op_map_empty_def op_map_empty_def lshm_invar_def
+  using assms by auto
+
+lemma lshm_bucket_update_map_of:
+  \<open>map_of (lshm_bucket_update k v b) = (map_of b)(k \<mapsto> v)\<close>
+  by (induction b rule: lshm_bucket_update.induct) auto
+
+lemma lshm_bucket_update_keys:
+  \<open>fst ` set (lshm_bucket_update k v b) = insert k (fst ` set b)\<close>
+  by (induction b rule: lshm_bucket_update.induct) auto
+
+lemma lshm_bucket_update_distinct:
+  \<open>distinct (map fst b) \<Longrightarrow> distinct (map fst (lshm_bucket_update k v b))\<close>
+  by (induction b rule: lshm_bucket_update.induct) (auto simp: lshm_bucket_update_keys)
+
+lemma lshm_bucket_update_set:
+  \<open>set (lshm_bucket_update k v b) \<subseteq> insert (k, v) (set b)\<close>
+  by (induction b rule: lshm_bucket_update.induct) auto
+
+lemma lshm_update_\<alpha>:
+  assumes I: \<open>lshm_invar xs\<close>
+  shows \<open>lshm_\<alpha> (lshm_op_map_update k v xs) = (lshm_\<alpha> xs)(k \<mapsto> v)\<close>
+proof (rule ext)
+  fix k'
+  from I have [simp]: \<open>0 < length xs\<close> unfolding lshm_invar_def by (cases xs) auto
+  show \<open>lshm_\<alpha> (lshm_op_map_update k v xs) k' = ((lshm_\<alpha> xs)(k \<mapsto> v)) k'\<close>
+  proof (cases \<open>lshm_bucket_of (length xs) k' = lshm_bucket_of (length xs) k\<close>)
+    case True
+    then show ?thesis
+      apply (auto simp: lshm_\<alpha>_def lshm_op_map_update_def Let_def lshm_bucket_of_def
+        lshm_bucket_update_map_of)
+      using \<open>0 < length xs\<close> lshm_bucket_update_map_of apply auto[1]
+      using \<open>0 < length xs\<close> lshm_bucket_update_map_of by auto
+  next
+    case False
+    then have \<open>k' \<noteq> k\<close> by auto
+    with False show ?thesis
+      by (auto simp: lshm_\<alpha>_def lshm_op_map_update_def Let_def lshm_bucket_of_def)
+  qed
+qed
+
+lemma lshm_update_invar:
+  assumes \<open>lshm_invar xs\<close>
+  shows \<open>lshm_invar (lshm_op_map_update k v xs)\<close>
+  using assms
+  unfolding lshm_invar_def lshm_op_map_update_def Let_def
+  apply (auto simp: nth_list_update lshm_bucket_update_distinct
+    dest!: set_mp[OF lshm_bucket_update_set])
+  apply (simp add: lshm_bucket_update_distinct nth_list_update')
+  by (smt (verit) case_prod_conv lshm_bucket_update_distinct
+    lshm_bucket_update_map_of map_of_eq_Some_iff map_upd_Some_unfold
+    nth_list_update_eq nth_list_update_neq)
+
+lemma lshm_update_fref:
+  \<open>(uncurry2 (RETURN ooo lshm_op_map_update), uncurry2 (RETURN ooo op_map_update))
+  \<in> Id \<times>\<^sub>r lshm_rel \<rightarrow>\<^sub>f \<langle>lshm_rel\<rangle>nres_rel\<close>
+  by (intro frefI nres_relI)
+    (auto simp: lshm_rel_def in_br_conv lshm_update_\<alpha> lshm_update_invar)
+
+lemma lshm_bucket_of_bound[simp]: \<open>0 < n \<Longrightarrow> lshm_bucket_of n k < n\<close>
+  by (simp add: lshm_bucket_of_def)
+
+lemma lshm_bucket_delete_map_of:
+  \<open>distinct (map fst b) \<Longrightarrow> map_of (lshm_bucket_delete k b) = (map_of b)(k := None)\<close>
+  apply (induction b rule: lshm_bucket_delete.induct)
+  subgoal by auto
+  subgoal by (auto simp: fun_upd_twist map_of_eq_None_iff)
+  done
+
+lemma lshm_bucket_delete_set: \<open>set (lshm_bucket_delete k b) \<subseteq> set b\<close>
+  by (induction b rule: lshm_bucket_delete.induct) auto
+
+lemma lshm_bucket_delete_keys: \<open>fst ` set (lshm_bucket_delete k b) \<subseteq> fst ` set b\<close>
+  using lshm_bucket_delete_set by (rule image_mono)
+
+lemma lshm_bucket_delete_distinct:
+  \<open>distinct (map fst b) \<Longrightarrow> distinct (map fst (lshm_bucket_delete k b))\<close>
+  by (induction b rule: lshm_bucket_delete.induct)
+    (auto dest!: set_mp[OF lshm_bucket_delete_keys])
+
+lemma lshm_delete_\<alpha>:
+  assumes I: \<open>lshm_invar xs\<close>
+  shows \<open>lshm_\<alpha> (lshm_op_map_delete k xs) = (lshm_\<alpha> xs)(k := None)\<close>
+proof (rule ext)
+  fix k'
+  from I have [simp]: \<open>0 < length xs\<close> unfolding lshm_invar_def by (cases xs) auto
+  from I have D: \<open>distinct (map fst (xs ! lshm_bucket_of (length xs) k))\<close>
+    unfolding lshm_invar_def by auto
+  show \<open>lshm_\<alpha> (lshm_op_map_delete k xs) k' = ((lshm_\<alpha> xs)(k := None)) k'\<close>
+  proof (cases \<open>lshm_bucket_of (length xs) k' = lshm_bucket_of (length xs) k\<close>)
+    case True
+    with D show ?thesis
+      apply (auto simp: lshm_\<alpha>_def lshm_op_map_delete_def Let_def lshm_bucket_delete_map_of)
+      subgoal using \<open>0 < length xs\<close> lshm_bucket_delete_map_of by fastforce
+      using \<open>0 < length xs\<close> lshm_bucket_delete_map_of by auto
+  next
+    case False
+    then have \<open>k' \<noteq> k\<close> by auto
+    with False show ?thesis
+      by (auto simp: lshm_\<alpha>_def lshm_op_map_delete_def Let_def)
+  qed
+qed
+
+lemma lshm_delete_invar:
+  assumes \<open>lshm_invar xs\<close>
+  shows \<open>lshm_invar (lshm_op_map_delete k xs)\<close>
+  using assms
+  unfolding lshm_invar_def lshm_op_map_delete_def Let_def
+  apply (auto simp: nth_list_update lshm_bucket_delete_distinct
+    dest!: set_mp[OF lshm_bucket_delete_set])
+  by (metis (mono_tags, lifting) case_prod_conv length_greater_0_conv
+    lshm_bucket_of_bound)
+
+lemma lshm_delete_fref:
+  \<open>(uncurry (RETURN oo lshm_op_map_delete), uncurry (RETURN oo op_map_delete))
+    \<in> Id \<times>\<^sub>r lshm_rel \<rightarrow>\<^sub>f \<langle>lshm_rel\<rangle>nres_rel\<close>
+  by (intro frefI nres_relI)
+    (auto simp: lshm_rel_def in_br_conv lshm_delete_\<alpha> lshm_delete_invar)
+
+lemma lshm_bucket_lookup_map_of[simp]:
+  \<open>lshm_bucket_lookup k b = map_of b k\<close>
+  by (induction b rule: lshm_bucket_lookup.induct) auto
+
+lemma lshm_bucket_contains_map_of[simp]:
+  \<open>lshm_bucket_contains k b \<longleftrightarrow> map_of b k \<noteq> None\<close>
+  by (induction b rule: lshm_bucket_contains.induct) auto
+
+lemma lshm_bucket_the_lookup_map_of:
+  \<open>map_of b k \<noteq> None \<Longrightarrow> lshm_bucket_the_lookup k b = the (map_of b k)\<close>
+  by (induction b rule: lshm_bucket_the_lookup.induct) (auto split: if_splits)
+
+lemma lshm_lookup_\<alpha>: \<open>lshm_op_map_lookup k xs = lshm_\<alpha> xs k\<close>
+  by (simp add: lshm_op_map_lookup_def lshm_\<alpha>_def Let_def)
+
+lemma lshm_lookup_fref:
+  \<open>(uncurry (RETURN oo lshm_op_map_lookup), uncurry (RETURN oo op_map_lookup))
+    \<in> Id \<times>\<^sub>r lshm_rel \<rightarrow>\<^sub>f \<langle>\<langle>Id\<rangle>option_rel\<rangle>nres_rel\<close>
+  by (intro frefI nres_relI)
+    (auto simp: lshm_rel_def in_br_conv lshm_lookup_\<alpha>)
+
+lemma lshm_contains_key_\<alpha>: \<open>lshm_op_map_contains_key k xs \<longleftrightarrow> lshm_\<alpha> xs k \<noteq> None\<close>
+  by (simp add: lshm_op_map_contains_key_def lshm_\<alpha>_def Let_def)
+
+lemma lshm_contains_key_fref:
+  \<open>(uncurry (RETURN oo lshm_op_map_contains_key), uncurry (RETURN oo op_map_contains_key))
+    \<in> Id \<times>\<^sub>r lshm_rel \<rightarrow>\<^sub>f \<langle>bool_rel\<rangle>nres_rel\<close>
+  by (intro frefI nres_relI)
+    (auto simp: lshm_rel_def in_br_conv lshm_contains_key_\<alpha> dom_def)
+
+lemma lshm_the_lookup_\<alpha>:
+  \<open>lshm_\<alpha> xs k \<noteq> None \<Longrightarrow> lshm_the_lookup k xs = the (lshm_\<alpha> xs k)\<close>
+  by (simp add: lshm_the_lookup_def lshm_\<alpha>_def Let_def lshm_bucket_the_lookup_map_of)
+
+lemma lshm_the_lookup_fref:
+  \<open>(uncurry (RETURN oo lshm_the_lookup), uncurry (RETURN oo op_map_the_lookup))
+    \<in> [\<lambda>(k,m). m k \<noteq> None]\<^sub>f Id \<times>\<^sub>r lshm_rel \<rightarrow> \<langle>Id\<rangle>nres_rel\<close>
+  by (intro frefI nres_relI)
+    (auto simp: lshm_rel_def in_br_conv lshm_the_lookup_\<alpha>)
+
+section \<open>Bucket-level Implemenations\<close>
+sepref_register "unat :: _ word \<Rightarrow> nat"
+lemma unat_word_refine[sepref_import_param]:
+  \<open>(id, unat) \<in> word_rel \<rightarrow> unat_rel' TYPE('a::len)\<close>
+  by (auto simp: unat_rel_def unat.rel_def in_br_conv)
+
+lemma lshm_bucket_of_alt:
+  \<open>lshm_bucket_of n k = op_unat_snat_conv (unat (khash k) mod op_snat_unat_conv n)\<close>
+  unfolding lshm_bucket_of_def by simp
+
+lemma mod_lt_boundI: \<open>0 < n \<Longrightarrow> n \<le> N \<Longrightarrow> (m::nat) mod n < N\<close>
+  by (meson mod_less_divisor less_le_trans)
+
+sepref_register khash lshm_bucket_of
+sepref_def lshm_bucket_of_impl is \<open>uncurry (RETURN oo PR_CONST lshm_bucket_of)\<close>
+  :: \<open>[\<lambda>(n,_). 0 < n]\<^sub>a (snat_assn' TYPE(64))\<^sup>k *\<^sub>a K\<^sup>k \<rightarrow> (snat_assn' TYPE(64))\<close>
+  unfolding PR_CONST_def lshm_bucket_of_alt
+  supply mod_lt_boundI[intro]
+  by sepref
+
+lemma box_assn_expand: \<open>\<upharpoonleft>(box_assn A) x p = (EXS c. \<upharpoonleft>ll_bpto c p ** A x c)\<close>
+  unfolding box_assn_def by simp
+
+subsection \<open>Bucket update\<close>
+
+definition lshm_bucket_update_impl
+  :: \<open>'ki \<Rightarrow> 'vi \<Rightarrow> ('ki \<times> 'vi ptr) cl_list \<Rightarrow> ('ki \<times> 'vi ptr) cl_list llM\<close>
+  where [llvm_code]:
+  \<open>lshm_bucket_update_impl ki vi \<equiv> MMonad.REC (\<lambda>f p.
+    if p = null then doM {
+      bv \<leftarrow> ll_ref vi;
+      ll_ref (Node (ki, bv) null)
+    }
+    else doM {
+      n \<leftarrow> ll_load p;
+      case node.val n of (kii, bv) \<Rightarrow> doM {
+        eq \<leftarrow> keq ki kii;
+        llc_if eq
+          (doM {
+            kfree ki; \<comment> \<open>the node keeps its key; the incoming one is freed\<close>
+            ov \<leftarrow> ll_load bv;
+            vfree ov;
+            ll_store vi bv;
+            Mreturn p
+          })
+          (doM {
+            tl \<leftarrow> f (node.next n);
+            ll_store (Node (kii, bv) tl) p;
+            Mreturn p
+          })
+      }
+    })\<close>
+
+lemmas lshm_bucket_update_impl_unfold =
+  REC_unfold_extr[OF lshm_bucket_update_impl_def, discharge_monos]
+
+lemma lshm_bucket_update_rule[vcg_rules]: \<open>llvm_htriple
+  (boxed_buckets_assn b bi ** K k ki ** V v vi)
+  (lshm_bucket_update_impl ki vi bi)
+  (\<lambda>r. boxed_buckets_assn (lshm_bucket_update k v b) r)\<close>
+proof (induction b arbitrary: bi)
+  case Nil
+  show ?case
+    apply (subst lshm_bucket_update_impl_unfold)
+    supply [simp] = cl_assn_simps box_assn_expand prod_assn_pair_conv sep_conj_exists
+    by vcg
+next
+  case (Cons e es)
+  obtain kc vc where [simp]: \<open>e = (kc, vc)\<close> by (cases e)
+  note [vcg_rules] = Cons.IH
+  show ?case
+    apply (subst lshm_bucket_update_impl_unfold)
+    supply [simp] = cl_assn_simps box_assn_expand prod_assn_pair_conv sep_conj_exists
+      bool.assn_def bool1_rel_def bool.rel_def in_br_conv pure_def from_bool_def
+    by vcg
+qed
+
+sepref_register lshm_bucket_update
+lemma lshm_bucket_update_hnr[sepref_fr_rules]:
+  \<open>(uncurry2 lshm_bucket_update_impl, uncurry2 (RETURN ooo lshm_bucket_update))
+    \<in> K\<^sup>d *\<^sub>a V\<^sup>d *\<^sub>a boxed_buckets_assn\<^sup>d \<rightarrow>\<^sub>a boxed_buckets_assn\<close>
+  by (sepref_to_hoare; vcg)
+
+subsection \<open>Bucket Delete\<close>
+
+definition lshm_bucket_delete_impl
+  :: \<open>'ki \<Rightarrow> ('ki \<times> 'vi ptr) cl_list \<Rightarrow> ('ki \<times> 'vi ptr) cl_list llM\<close>
+  where [llvm_code]:
+  \<open>lshm_bucket_delete_impl ki \<equiv> MMonad.REC (\<lambda> f p. doM {
+    if p = null then Mreturn null
+    else doM {
+      n \<leftarrow> ll_load p;
+      case node.val n of (kii, bv) \<Rightarrow> doM {
+        eq \<leftarrow> keq ki kii;
+        llc_if eq (doM {
+          kfree kii;
+          box_free vfree bv;
+          ll_free p;
+          Mreturn (node.next n)
+        }) (doM {
+          tl \<leftarrow> f (node.next n);
+          ll_store (Node (kii, bv) tl) p;
+          Mreturn p
+        })
+      }
+    }
+  })\<close>
+
+lemmas lshm_bucket_delete_impl_unfold =
+  REC_unfold_extr[OF lshm_bucket_delete_impl_def, discharge_monos]
+
+lemma lshm_bucket_delete_rule[vcg_rules]: \<open>llvm_htriple
+  (boxed_buckets_assn b bi ** K k ki)
+  (lshm_bucket_delete_impl ki bi)
+  (\<lambda>r. K k ki ** boxed_buckets_assn (lshm_bucket_delete k b) r)\<close>
+proof (induction b arbitrary: bi)
+  case Nil
+  then show ?case
+    apply (subst lshm_bucket_delete_impl_unfold)
+    supply [simp] = cl_assn_simps sep_conj_exists Nil
+    by vcg
+next
+  case (Cons e es)
+  obtain kc vc where [simp]: \<open>e = (kc, vc)\<close> by (cases e)
+  note [vcg_rules] = Cons.IH MK_FREED[OF box_free_rule[OF val.afree_free]]
+  show ?case
+    apply (subst lshm_bucket_delete_impl_unfold)
+    supply [simp] = cl_assn_simps prod_assn_pair_conv sep_conj_exists
+      bool.assn_def bool1_rel_def bool.rel_def in_br_conv pure_def from_bool_def
+    by vcg
+qed
+
+sepref_register lshm_bucket_delete
+lemma lshm_bucket_delete_hnr[sepref_fr_rules]:
+  \<open>(uncurry lshm_bucket_delete_impl, uncurry (RETURN oo lshm_bucket_delete))
+  \<in> K\<^sup>k *\<^sub>a boxed_buckets_assn\<^sup>d \<rightarrow>\<^sub>a boxed_buckets_assn\<close>
+  by (sepref_to_hoare; vcg)
+
+subsection \<open>Bucket Contains\<close>
+
+definition \<open>lshm_bucket_contains_fold_inner x \<equiv> \<lambda>acc (k,v). acc \<or> (x = k)\<close> 
+
+lemma lshm_bucket_contains_fold:
+  \<open>lshm_bucket_contains k xs = foldl (lshm_bucket_contains_fold_inner k) False xs\<close>
+  unfolding lshm_bucket_contains_fold_inner_def
+  by (induction xs; auto simp: rev_induct)
+
+definition lshm_bucket_contains_step where [llvm_code, llvm_inline]:
+  \<open>lshm_bucket_contains_step ki \<equiv> \<lambda>acci (kii, bv). doM {
+    eq \<leftarrow> keq ki kii;
+    ll_or acci eq
+  }\<close>
+
+lemma lshm_bucket_contains_step_rule: \<open>llvm_htriple
+  ((K k ki ** bool1_assn a ai) ** boxed_bucket_assn x xi)
+  (lshm_bucket_contains_step ki ai xi)
+  (\<lambda>r. (K k ki ** bool1_assn (lshm_bucket_contains_fold_inner k a x) r) ** boxed_bucket_assn x xi)\<close>
+  unfolding lshm_bucket_contains_step_def lshm_bucket_contains_fold_inner_def
+  apply (cases x; cases xi; simp only: prod_assn_pair_conv prod.case)
+  supply [simp] = bool.assn_def bool1_rel_def bool.rel_def in_br_conv pure_def from_bool_def
+  by vcg
+
+definition lshm_bucket_contains_impl :: \<open>'ki \<Rightarrow> ('ki \<times> 'vi ptr) cl_list \<Rightarrow> 1 word llM\<close>
+  where [llvm_code]:
+  \<open>lshm_bucket_contains_impl ki p \<equiv> cl_fold' (lshm_bucket_contains_step ki) 0 p\<close>
+
+lemma lshm_bucket_contains_rule[vcg_rules]: \<open>llvm_htriple
+  (boxed_buckets_assn b bi ** K k ki)
+  (lshm_bucket_contains_impl ki bi)
+  (\<lambda>r. boxed_buckets_assn b bi ** K k ki ** bool1_assn (lshm_bucket_contains k b) r)\<close>
+  unfolding lshm_bucket_contains_impl_def lshm_bucket_contains_fold
+  supply [vcg_rules] = cl_fold'_rule[where R = \<open>\<lambda>a ai. K k ki ** bool1_assn a ai\<close>
+    and A = boxed_bucket_assn and fa = \<open>lshm_bucket_contains_fold_inner k\<close>
+    and a = False, OF lshm_bucket_contains_step_rule]
+  supply [simp] = bool1_rel_def bool.rel_def in_br_conv pure_def
+  by vcg
+
+sepref_register lshm_bucket_contains
+lemma lshm_bucket_contains_hnr[sepref_fr_rules]:
+  \<open>(uncurry lshm_bucket_contains_impl, uncurry (RETURN oo lshm_bucket_contains))
+  \<in> K\<^sup>k *\<^sub>a boxed_buckets_assn\<^sup>k \<rightarrow>\<^sub>a bool1_assn\<close>
+  supply [simp] = bool1_rel_def bool.rel_def in_br_conv pure_def
+  by (sepref_to_hoare; vcg)
+
+subsection \<open>Bucket Lookup\<close>
+
+definition lshm_bucket_lookup_impl
+  :: \<open>'ki \<Rightarrow> ('ki \<times> 'vi ptr) cl_list \<Rightarrow> 'vi ptr llM\<close> where [llvm_code]:
+  \<open>lshm_bucket_lookup_impl ki \<equiv> MMonad.REC (\<lambda>f p.
+  if p = null then Mreturn null
+  else doM {
+    n \<leftarrow> ll_load p;
+    case node.val n of (kii, bv) \<Rightarrow> doM {
+      eq \<leftarrow> keq ki kii;
+      llc_if eq (doM {
+        ov \<leftarrow> ll_load bv;
+        v \<leftarrow> vcopy ov;
+        ll_ref v
+      }) (f (node.next n))
+    }
+  })\<close>
+
+lemmas lshm_bucket_lookup_impl_unfold =
+  REC_unfold_extr[OF lshm_bucket_lookup_impl_def, discharge_monos]
+
+lemma lshm_bucket_lookup_rule[vcg_rules]: \<open>llvm_htriple
+  (boxed_buckets_assn b bi ** K k ki)
+  (lshm_bucket_lookup_impl ki bi)
+  (\<lambda>r. boxed_buckets_assn b bi ** K k ki ** vopt_assn (lshm_bucket_lookup k b) r)\<close>
+proof (induction b arbitrary: bi)
+  case Nil
+  then show ?case
+    apply (subst lshm_bucket_lookup_impl_unfold)
+    supply [simp] = cl_assn_simps sep_conj_exists
+    by vcg
+next
+  case (Cons e es)
+  obtain kc vc where [simp]: \<open>e = (kc, vc)\<close> by (cases e)
+  note [vcg_rules] = Cons.IH
+  show ?case
+    apply (subst lshm_bucket_lookup_impl_unfold)
+    supply [simp] = cl_assn_simps box_assn_expand prod_assn_pair_conv sep_conj_exists
+      bool.assn_def bool1_rel_def bool.rel_def in_br_conv pure_def from_bool_def
+    by vcg
+qed
+
+sepref_register lshm_bucket_lookup
+lemma lshm_bucket_lookup_hnr[sepref_fr_rules]:
+  \<open>(uncurry lshm_bucket_lookup_impl, uncurry (RETURN oo lshm_bucket_lookup))
+  \<in> K\<^sup>k *\<^sub>a boxed_buckets_assn\<^sup>k \<rightarrow>\<^sub>a vopt_assn\<close>
+  by (sepref_to_hoare; vcg)
+
+subsection \<open>Bucket the Lookup\<close>
+
+definition lshm_bucket_the_lookup_impl
+  :: \<open>'ki \<Rightarrow> ('ki \<times> 'vi ptr) cl_list \<Rightarrow> 'vi llM\<close> where[llvm_code]:
+  \<open>lshm_bucket_the_lookup_impl ki p \<equiv> doM {
+    vp \<leftarrow> lshm_bucket_lookup_impl ki p;
+    v \<leftarrow> ll_load vp;
+    ll_free vp;
+    Mreturn v
+  }\<close>
+
+lemma lshm_bucket_the_lookup_rule[vcg_rules]:
+  assumes \<open>lshm_bucket_contains k b\<close>
+  shows \<open>llvm_htriple (boxed_buckets_assn b bi ** K k ki)
+  (lshm_bucket_the_lookup_impl ki bi)
+  (\<lambda>r. boxed_buckets_assn b bi ** K k ki ** V (lshm_bucket_the_lookup k b) r)\<close>
+proof -
+  from assms obtain v where [simp]: \<open>map_of b k = Some v\<close> by auto
+  show ?thesis
+    unfolding lshm_bucket_the_lookup_impl_def
+    supply [simp] = lshm_bucket_the_lookup_map_of box_assn_expand sep_conj_exists
+    by vcg
+qed
+
+sepref_register lshm_bucket_the_lookup
+lemma lshm_bucket_the_lookup_hnr[sepref_fr_rules]:
+  \<open>(uncurry lshm_bucket_the_lookup_impl, uncurry (RETURN oo lshm_bucket_the_lookup))
+  \<in> [\<lambda>(k, b). lshm_bucket_contains k b]\<^sub>a K\<^sup>k *\<^sub>a boxed_buckets_assn\<^sup>k \<rightarrow> V\<close>
+  by (sepref_to_hoare; vcg)
+
+section \<open>Hashmap Implementation\<close>
+
+text \<open>We use @{term oelem_assn} from Isabelle_LLVM.Proto_EOArray to temporarily move elements out of arrays.
+  Note that this only applies to reasoning, we don't actually implement an option type for buckets
+  (unlike for the values inside the bucket tuples, where we actually use a box).\<close>
+definition hm_assn' :: \<open>(('k \<times> 'v) list option list, 64 word \<times> 64 word \<times> ('ki \<times> 'vi ptr) node ptr ptr) dr_assn\<close> where
+  \<open>hm_assn' \<equiv> mk_assn (\<lambda>xs ali. EXS xsi. \<upharpoonleft>arl_assn xsi ali ** \<upharpoonleft>(list_assn (oelem_assn (mk_assn boxed_buckets_assn))) xs xsi)\<close>
+
+definition hm_opt_rel :: \<open>(('k \<times> 'v) list option list \<times> ('k, 'v) hashmap) set\<close> where
+  \<open>hm_opt_rel \<equiv> br (map the) (\<lambda>xs. None \<notin> set xs)\<close>
+
+lemma in_hm_opt_rel_conv:
+  \<open>(xs', xs) \<in> hm_opt_rel \<longleftrightarrow> xs = map the xs' \<and> None \<notin> set xs'\<close>
+  unfolding hm_opt_rel_def by (simp add: in_br_conv)
+
+definition hm_assn''
+  :: \<open>('k, 'v) hashmap \<Rightarrow> 64 word \<times> 64 word \<times> ('ki \<times> 'vi ptr) node ptr ptr \<Rightarrow> assn\<close> where
+  \<open>hm_assn'' \<equiv> hr_comp (\<upharpoonleft>hm_assn') hm_opt_rel\<close>
+
+lemma hm_assn''_expand:
+  \<open>hm_assn'' xs c = (EXS xs'. \<upharpoonleft>hm_assn' xs' c ** \<up>((xs', xs) \<in> hm_opt_rel))\<close>
+  by (simp add: hm_assn''_def hr_comp_def)
+
+lemma hm_opt_rel_length: \<open>(xs', xs) \<in> hm_opt_rel \<Longrightarrow> length xs' = length xs\<close>
+  by (auto simp: in_hm_opt_rel_conv)
+
+lemma hm_opt_rel_nth:
+  assumes R: \<open>(xs', xs) \<in> hm_opt_rel\<close> and I: \<open>i < length xs\<close>
+  shows \<open>xs' ! i = Some (xs ! i)\<close>
+proof -
+  from R have M: \<open>xs = map the xs'\<close> and N: \<open>None \<notin> set xs'\<close>
+    by (auto simp: in_hm_opt_rel_conv)
+  from I M have L: \<open>i < length xs'\<close> by simp
+  with N have \<open>xs' ! i \<noteq> None\<close> using nth_mem by metis
+  with L show ?thesis unfolding M by (cases \<open>xs' ! i\<close>) auto
+qed
+
+lemma hm_opt_rel_upd:
+  \<open>(xs', xs) \<in> hm_opt_rel \<Longrightarrow> (xs'[i := Some b], xs[i := b]) \<in> hm_opt_rel\<close>
+  by (auto simp: in_hm_opt_rel_conv map_update
+    dest!: subsetD[OF set_update_subset_insert])
+
+lemma hm_opt_rel_replicate: \<open>(replicate n (Some b), replicate n b) \<in> hm_opt_rel\<close>
+  by (auto simp: in_hm_opt_rel_conv)
+
+(* Pretty much copied from Proto_EOArray.thy *)
+lemma hm_nth_rule[vcg_rules]: "llvm_htriple 
+  (\<upharpoonleft>hm_assn' xs p \<and>* \<upharpoonleft>snat.assn i ii \<and>* \<up>\<^sub>d(i < length xs \<and> xs!i\<noteq>None)) 
+  (arl_nth p ii)
+  (\<lambda>ri. boxed_buckets_assn (the (xs!i)) ri \<and>* \<upharpoonleft>hm_assn' (xs[i:=None]) p)"  
+  unfolding hm_assn'_def 
+  supply [simp] = lo_extract_elem
+  apply vcg
+  done
+
+lemma hm_upd_rule_snat[vcg_rules]: "llvm_htriple 
+  (\<upharpoonleft>hm_assn' xs p \<and>* boxed_buckets_assn x xi \<and>* \<upharpoonleft>snat.assn i ii \<and>* \<up>\<^sub>d(i < length xs \<and> xs!i=None)) 
+  (arl_upd p ii xi)
+  (\<lambda>r. \<up>(r = p) \<and>* \<upharpoonleft>hm_assn' (xs[i := Some x]) p)"
+  unfolding hm_assn'_def
+  supply [simp] = lo_insert_elem
+  apply vcg
+  done
+
+lemma hm_len_rule[vcg_rules]: \<open>llvm_htriple
+  (\<upharpoonleft>hm_assn' xs p)
+  (arl_len p)
+  (\<lambda>r. \<upharpoonleft>hm_assn' xs p ** \<upharpoonleft>snat.assn (length xs) r)\<close>
+  unfolding hm_assn'_def
+  apply vcg
+  apply (auto simp: sep_algebra_simps ENTAILS_def entails_def)
+  by (smt (verit, del_insts) extract_pure_assn list_assn_neq_len(2)
+    pure_true_conv sep.mult_commute sep_conj_empty sep_conj_false_left
+    snat.assn_pure)
+
+lemma lshm_bucket_of_impl_rule[vcg_rules]:
+  assumes \<open>0 < n\<close>
+  shows \<open>llvm_htriple
+    (\<upharpoonleft>snat.assn n ni ** K k ki)
+    (lshm_bucket_of_impl ni ki)
+    (\<lambda>r. \<upharpoonleft>snat.assn n ni ** K k ki ** \<upharpoonleft>snat.assn (lshm_bucket_of n k) r)\<close>
+proof -
+  have PRE: \<open>(\<lambda>(n, _). 0 < n) (n, k)\<close> using assms by simp
+  note HT = hfref_htriple_k1_k2_guard[OF lshm_bucket_of_impl.refine PRE,
+    unfolded PR_CONST_def]
+  show ?thesis
+    using HT by (simp add: snat_rel_def snat.assn_is_rel[symmetric])
+qed
+
+subsection \<open>Update\<close>
+
+definition \<open>lshm_op_map_update_impl \<equiv> \<lambda>ki vi xsi. doM {
+    l \<leftarrow> arl_len xsi;
+    bii \<leftarrow> lshm_bucket_of_impl l ki;
+    bi \<leftarrow> arl_nth xsi bii; 
+    bi \<leftarrow> lshm_bucket_update_impl ki vi bi;
+    arl_upd xsi bii bi 
+  }\<close>
+
+lemma lshm_op_map_update_rule[vcg_rules]: \<open>llvm_htriple
+  (K k ki ** V v vi ** hm_assn'' xs xsi ** \<up>\<^sub>d(xs \<noteq> []))
+  (lshm_op_map_update_impl ki vi xsi)
+  (\<lambda>r. hm_assn'' (lshm_op_map_update k v xs) r)\<close>
+  unfolding lshm_op_map_update_impl_def hm_assn''_expand
+  supply [simp] = hm_opt_rel_length hm_opt_rel_nth hm_opt_rel_upd
+    lshm_op_map_update_def Let_def sep_conj_exists
+  by vcg
+
+lemma lshm_op_map_update_hnr:
+  \<open>(uncurry2 lshm_op_map_update_impl, uncurry2 (RETURN ooo lshm_op_map_update))
+  \<in> [\<lambda>((k,v),xs). xs\<noteq>[]]\<^sub>a K\<^sup>d *\<^sub>a V\<^sup>d *\<^sub>a hm_assn''\<^sup>d \<rightarrow> hm_assn''\<close>
+  apply (sepref_to_hoare; vcg)
+  done
+
+lemma lshm_rel_nonempty[fcomp_prenorm_simps]: \<open>(xs', m) \<in> lshm_rel \<Longrightarrow> xs' \<noteq> []\<close>
+  by (auto simp: lshm_rel_def in_br_conv lshm_invar_def)
+
+lemmas lshm_update_hnr[sepref_fr_rules] =
+  lshm_op_map_update_hnr[FCOMP lshm_update_fref]
+
+subsection \<open>Delete\<close>
+
+definition \<open>lshm_op_map_delete_impl \<equiv> \<lambda>ki xsi. doM {
+    l \<leftarrow> arl_len xsi;
+    bii \<leftarrow> lshm_bucket_of_impl l ki;
+    bi \<leftarrow> arl_nth xsi bii; 
+    bi \<leftarrow> lshm_bucket_delete_impl ki bi;
+    arl_upd xsi bii bi   
+  }\<close>
+
+lemma lshm_op_map_delete_rule[vcg_rules]: \<open>llvm_htriple
+  (K k ki ** hm_assn'' xs xsi ** \<up>\<^sub>d(xs \<noteq> []))
+  (lshm_op_map_delete_impl ki xsi)
+  (\<lambda>r. K k ki ** hm_assn'' (lshm_op_map_delete k xs) r)\<close>
+  unfolding lshm_op_map_delete_impl_def hm_assn''_expand
+  supply [simp] = hm_opt_rel_length hm_opt_rel_nth hm_opt_rel_upd
+    lshm_op_map_delete_def Let_def sep_conj_exists
+  by vcg
+
+lemma lshm_op_map_delete_hnr:
+  \<open>(uncurry lshm_op_map_delete_impl, uncurry (RETURN oo lshm_op_map_delete))
+  \<in> [\<lambda>(k,xs). xs\<noteq>[]]\<^sub>a K\<^sup>k *\<^sub>a hm_assn''\<^sup>d \<rightarrow> hm_assn''\<close>
+  apply (sepref_to_hoare; vcg)
+  done
+
+lemmas lshm_delete_hnr[sepref_fr_rules] = 
+  lshm_op_map_delete_hnr[FCOMP lshm_delete_fref]
+
+subsection \<open>Contains\<close>
+
+lemma hm_opt_rel_restore:
+  \<open>(xs', xs) \<in> hm_opt_rel \<Longrightarrow> i < length xs \<Longrightarrow> xs'[i := Some (xs ! i)] = xs'\<close>
+  by (metis hm_opt_rel_nth list_update_id)
+
+definition \<open>lshm_op_map_contains_key_impl \<equiv> \<lambda>ki xsi. doM {
+    l \<leftarrow> arl_len xsi;
+    bii \<leftarrow> lshm_bucket_of_impl l ki;
+    bi \<leftarrow> arl_nth xsi bii;
+    r \<leftarrow> lshm_bucket_contains_impl ki bi;
+    arl_upd xsi bii bi;
+    Mreturn r
+  }\<close>
+
+lemma lshm_op_map_contains_key_rule[vcg_rules]: \<open>llvm_htriple
+  (K k ki ** hm_assn'' xs xsi ** \<up>\<^sub>d(xs \<noteq> []))
+  (lshm_op_map_contains_key_impl ki xsi)
+  (\<lambda>r. K k ki ** hm_assn'' xs xsi ** bool1_assn (lshm_op_map_contains_key k xs) r)\<close>
+  unfolding lshm_op_map_contains_key_impl_def hm_assn''_expand
+  supply [simp] = hm_opt_rel_length hm_opt_rel_nth hm_opt_rel_restore
+    lshm_op_map_contains_key_def Let_def sep_conj_exists
+  by vcg
+
+lemma lshm_op_map_contains_key_hnr:
+  \<open>(uncurry lshm_op_map_contains_key_impl, uncurry (RETURN oo lshm_op_map_contains_key))
+  \<in> [\<lambda>(k,xs). xs\<noteq>[]]\<^sub>a K\<^sup>k *\<^sub>a hm_assn''\<^sup>k \<rightarrow> bool1_assn\<close>
+  supply [simp] = bool1_rel_def bool.rel_def in_br_conv pure_def
+  by (sepref_to_hoare; vcg)
+
+lemmas lshm_contains_key_hnr[sepref_fr_rules] =
+  lshm_op_map_contains_key_hnr[FCOMP lshm_contains_key_fref]
+
+subsection \<open>Lookup\<close>
+
+definition \<open>lshm_op_map_lookup_impl \<equiv> \<lambda>ki xsi. doM {
+    l \<leftarrow> arl_len xsi;
+    bii \<leftarrow> lshm_bucket_of_impl l ki;
+    bi \<leftarrow> arl_nth xsi bii;
+    r \<leftarrow> lshm_bucket_lookup_impl ki bi;
+    arl_upd xsi bii bi;
+    Mreturn r
+  }\<close>
+
+lemma lshm_op_map_lookup_rule[vcg_rules]: \<open>llvm_htriple
+  (K k ki ** hm_assn'' xs xsi ** \<up>\<^sub>d(xs \<noteq> []))
+  (lshm_op_map_lookup_impl ki xsi)
+  (\<lambda>r. K k ki ** hm_assn'' xs xsi ** vopt_assn (lshm_op_map_lookup k xs) r)\<close>
+  unfolding lshm_op_map_lookup_impl_def hm_assn''_expand
+  supply [simp] = hm_opt_rel_length hm_opt_rel_nth hm_opt_rel_restore
+    lshm_op_map_lookup_def Let_def sep_conj_exists
+  by vcg
+
+lemma lshm_op_map_lookup_hnr:
+  \<open>(uncurry lshm_op_map_lookup_impl, uncurry (RETURN oo lshm_op_map_lookup))
+  \<in> [\<lambda>(k,xs). xs\<noteq>[]]\<^sub>a K\<^sup>k *\<^sub>a hm_assn''\<^sup>k \<rightarrow> vopt_assn\<close>
+  by (sepref_to_hoare; vcg)
+
+lemmas lshm_lookup_hnr[sepref_fr_rules] =
+  lshm_op_map_lookup_hnr[FCOMP lshm_lookup_fref]
+
+subsection \<open>The-Lookup\<close>
+
+definition \<open>lshm_the_lookup_impl \<equiv> \<lambda>ki xsi. doM {
+    l \<leftarrow> arl_len xsi;
+    bii \<leftarrow> lshm_bucket_of_impl l ki;
+    bi \<leftarrow> arl_nth xsi bii;
+    r \<leftarrow> lshm_bucket_the_lookup_impl ki bi;
+    arl_upd xsi bii bi;
+    Mreturn r
+  }\<close>
+
+lemma lshm_the_lookup_rule[vcg_rules]: \<open>llvm_htriple
+  (K k ki ** hm_assn'' xs xsi ** \<up>\<^sub>d(xs \<noteq> [] \<and> lshm_op_map_contains_key k xs))
+  (lshm_the_lookup_impl ki xsi)
+  (\<lambda>r. K k ki ** hm_assn'' xs xsi ** V (lshm_the_lookup k xs) r)\<close>
+  unfolding lshm_the_lookup_impl_def hm_assn''_expand
+  supply [simp] = hm_opt_rel_length hm_opt_rel_nth hm_opt_rel_restore
+    lshm_the_lookup_def lshm_op_map_contains_key_def Let_def sep_conj_exists
+  by vcg
+
+lemma lshm_the_lookup_impl_hnr:
+  \<open>(uncurry lshm_the_lookup_impl, uncurry (RETURN oo lshm_the_lookup))
+  \<in> [\<lambda>(k,xs). xs\<noteq>[] \<and> lshm_op_map_contains_key k xs]\<^sub>a K\<^sup>k *\<^sub>a hm_assn''\<^sup>k \<rightarrow> V\<close>
+  by (sepref_to_hoare; vcg)
+
+lemma lshm_rel_contains[fcomp_prenorm_simps]:
+  \<open>(xs', m) \<in> lshm_rel \<Longrightarrow> lshm_op_map_contains_key k xs' \<longleftrightarrow> m k \<noteq> None\<close>
+  by (auto simp: lshm_rel_def in_br_conv lshm_contains_key_\<alpha>)
+
+lemmas lshm_the_lookup_hnr[sepref_fr_rules] =
+  lshm_the_lookup_impl_hnr[FCOMP lshm_the_lookup_fref]
+
+subsection \<open>Empty\<close>
+
+definition lshm_empty :: \<open>64 word \<Rightarrow> (64 word \<times> 64 word \<times> ('ki \<times> 'vi ptr) node ptr ptr) llM\<close>
+  where [llvm_code, llvm_inline]:
+  \<open>lshm_empty ni \<equiv> arl_new_repl_init TYPE(('ki \<times> 'vi ptr) node ptr) ni\<close>
+
+lemma list_assn_oelem_replicate_empty[simp]:
+  \<open>\<upharpoonleft>(list_assn (oelem_assn (mk_assn boxed_buckets_assn))) (replicate n (Some [])) (replicate n init) = \<box>\<close>
+  by (induction n) (auto simp: sep_algebra_simps cl_assn_simps(1))
+
+lemma lshm_empty_aux_rule:
+  \<open>llvm_htriple
+    (\<upharpoonleft>snat.assn n ni)
+    (lshm_empty ni)
+    (\<lambda>r. \<upharpoonleft>hm_assn' (replicate n (Some [])) r)\<close>
+  unfolding lshm_empty_def hm_assn'_def
+  apply vcg
+  apply (auto simp: sep_algebra_simps ENTAILS_def entails_def)
+  by (metis init_ptr_def list_assn_oelem_replicate_empty sep_conj_empty)
+
+lemma lshm_empty_rule[vcg_rules]:
+  \<open>llvm_htriple
+    (\<upharpoonleft>snat.assn n ni)
+    (lshm_empty ni)
+    (\<lambda>r. hm_assn'' (lshm_op_map_empty n) r)\<close>
+  unfolding hm_assn''_expand lshm_op_map_empty_def
+  supply [vcg_rules] = lshm_empty_aux_rule
+  supply [simp] = hm_opt_rel_replicate
+  by vcg
+
+subsection \<open>Free\<close>
+
+text \<open>\<open>nulled_prefix\<close> and its bookkeeping are redefined here because the
+  originals are scoped inside the \<open>array_pmap\<close> locale of \<open>IICF_PartialMap\<close>.\<close>
+
+definition \<open>nulled_prefix (xs :: 'c option list) i = replicate i None @ drop i xs\<close>
+
+lemma nulled_emp[simp]: \<open>nulled_prefix xs 0 = xs\<close>
+  unfolding nulled_prefix_def by simp
+
+lemma nulled_prefix_length[simp]:
+  \<open>i \<le> length xs \<Longrightarrow> length (nulled_prefix xs i) = length xs\<close>
+  unfolding nulled_prefix_def by simp
+
+lemma nulled_prefix_nth[simp]:
+  \<open>i < length xs \<Longrightarrow> nulled_prefix xs i ! i = xs ! i\<close>
+  unfolding nulled_prefix_def
+  by (metis Cons_nth_drop_Suc drop_append_miracle length_replicate nth_via_drop)
+
+lemma nulled_prefix_step[simp]:
+  \<open>i < length xs \<Longrightarrow> (nulled_prefix xs i)[i := Option.None] = nulled_prefix xs (Suc i)\<close>
+  unfolding nulled_prefix_def
+  by (metis Cons_nth_drop_Suc append_Cons length_replicate
+            list_update_length replicate_Suc replicate_app_Cons_same)
+
+lemma nulled_prefix_full[simp]:
+  \<open>nulled_prefix xs (length xs) = replicate (length xs) Option.None\<close>
+  unfolding nulled_prefix_def by simp
+
+definition lshm_free :: \<open>64 word \<times> 64 word \<times> ('ki \<times> 'vi ptr) node ptr ptr \<Rightarrow> unit llM\<close>
+  where [llvm_code]:
+  \<open>lshm_free xsi \<equiv> doM {
+    llc_while
+      (\<lambda>i. doM { l \<leftarrow> arl_len xsi; ll_icmp_ult i l })
+      (\<lambda>i. doM {
+        bi \<leftarrow> arl_nth xsi i;
+        bucket.cl_free bi;
+        i \<leftarrow> ll_add i (signed_nat 1);
+        Mreturn i
+      }) (signed_nat 0);
+    arl_free xsi
+  }\<close>
+
+lemma all_some_nth: \<open>None \<notin> set xs \<Longrightarrow> i < length xs \<Longrightarrow> xs ! i \<noteq> None\<close>
+  by (metis nth_mem)
+
+lemma list_assn_oelem_all_None:
+  \<open>set xs \<subseteq> {None} \<Longrightarrow>
+    \<upharpoonleft>(list_assn (oelem_assn A)) xs xsi = \<up>(length xsi = length xs)\<close>
+proof (induction xs arbitrary: xsi)
+  case Nil
+  then show ?case by (cases xsi) (auto simp: sep_algebra_simps)
+next
+  case (Cons x xs)
+  then show ?case
+    by (cases xsi) (auto simp: sep_algebra_simps list_assn_cons1_conv Cons.IH)
+qed
+
+text \<open>Once all slots are freed, the remaining \<open>hm_assn'\<close> is just the raw array.\<close>
+lemma lshm_free_arl_rule[vcg_rules]:
+  \<open>llvm_htriple (\<upharpoonleft>hm_assn' xs ali ** \<up>\<^sub>d(set xs \<subseteq> {None})) (arl_free ali) (\<lambda>_. \<box>)\<close>
+  unfolding hm_assn'_def
+  supply [simp] = list_assn_oelem_all_None sep_conj_exists
+  by vcg
+
+lemma lshm_free_aux_rule:
+  \<open>llvm_htriple
+    (\<upharpoonleft>hm_assn' xs' ali ** \<up>\<^sub>d(None \<notin> set xs'))
+    (lshm_free ali)
+    (\<lambda>_. \<box>)\<close>
+  unfolding lshm_free_def
+  apply (rewrite annotate_llc_while[where
+    I=\<open>\<lambda>ii t. EXS i. \<upharpoonleft>snat.assn i ii ** \<upharpoonleft>hm_assn' (nulled_prefix xs' i) ali
+        ** \<up>(i \<le> length xs' \<and> None \<notin> set xs') ** \<up>\<^sub>!(t = length xs' - i)\<close>
+    and R=\<open>less_than\<close>])
+  supply [simp] = all_some_nth
+  apply vcg_monadify
+  apply vcg'
+  done
+
+lemma lshm_free_rule[vcg_rules]:
+  \<open>llvm_htriple (hm_assn'' xs ali) (lshm_free ali) (\<lambda>_. \<box>)\<close>
+  unfolding hm_assn''_expand
+  supply [vcg_rules] = lshm_free_aux_rule
+  supply [simp] = in_hm_opt_rel_conv sep_conj_exists
+  by vcg
+
+lemma lshm_free_mk_free[sepref_frame_free_rules]: \<open>MK_FREE hm_assn'' lshm_free\<close>
+  by (rule MK_FREEI) (rule lshm_free_rule)
+
+text \<open>Convenient top-level assertion for outside use\<close>
+abbreviation \<open>hm_assn \<equiv> hr_comp hm_assn'' lshm_rel\<close>
+
+end
+
+end
