PAC_Checker_LLVM/More_EOArray.thy
@@ -1,0 +1,250 @@
+theory More_EOArray
+  imports Isabelle_LLVM.Proto_EOArray
+    LLVM_String
+begin
+
+text \<open>This theory contains a variation of @{term nao_assn} that stores elements directly
+  instead of wrappig them in @{term option}. Also, we store the length and capacity like for
+  @{term arl_assn}. Noteworthably, this is an opinionated implementation that will copy elements on retreival.
+  \<close>
+
+context copyable_assn
+begin
+
+definition oa_assn :: "('a list, ('b, 64) array_list) dr_assn" where
+  \<open>oa_assn \<equiv> mk_assn (\<lambda>xs ali. EXS xsi. \<upharpoonleft>arl_assn xsi ali ** \<upharpoonleft>(list_assn (mk_assn A)) xs xsi)\<close>
+abbreviation \<open>oa_assn' \<equiv> \<upharpoonleft>oa_assn\<close>
+
+section \<open>nth\<close>
+
+definition oa_nth :: \<open>('b, 64) array_list \<Rightarrow> 64 word \<Rightarrow> 'b llM\<close> where[llvm_code,llvm_inline]:
+  \<open>oa_nth ai i \<equiv> doM {xi \<leftarrow> arl_nth ai i; acopy xi}\<close>
+
+lemma list_assn_focus:
+  assumes I: \<open>i < length xs\<close>
+  shows \<open>\<upharpoonleft>(list_assn (mk_assn A)) xs xsi =
+    (A (xs!i) (xsi!i)
+     ** \<upharpoonleft>(list_assn (mk_assn A)) (take i xs) (take i xsi)
+     ** \<upharpoonleft>(list_assn (mk_assn A)) (drop (Suc i) xs) (drop (Suc i) xsi)
+     ** \<up>(length xsi = length xs))\<close>
+proof (cases \<open>length xsi = length xs\<close>)
+  case True
+  obtain xs\<^sub>1 x xs\<^sub>2 where XSF: \<open>xs = xs\<^sub>1 @ x # xs\<^sub>2\<close> and LEN1: \<open>i = length xs\<^sub>1\<close>
+    using id_take_nth_drop[OF I] I by fastforce
+  obtain ys\<^sub>1 y ys\<^sub>2 where YSF: \<open>xsi = ys\<^sub>1 @ y # ys\<^sub>2\<close> and LEN2: \<open>length ys\<^sub>1 = length xs\<^sub>1\<close>
+    and LEN3: \<open>length ys\<^sub>2 = length xs\<^sub>2\<close>
+    using split_list_according[OF XSF True] .
+  show ?thesis
+    unfolding XSF YSF LEN1
+    by (simp add: LEN2 LEN3 nth_append sep_algebra_simps sep_conj_c)
+qed (simp add: sep_algebra_simps)
+
+lemma list_assn_acopy_nth_rule[vcg_rules]:
+  \<open>llvm_htriple
+     (\<upharpoonleft>(list_assn (mk_assn A)) xs xsi ** \<up>\<^sub>d(i < length xs))
+     (acopy (xsi!i))
+     (\<lambda>r. \<upharpoonleft>(list_assn (mk_assn A)) xs xsi ** A (xs!i) r)\<close>
+proof (induction xs arbitrary: i xsi)
+  case Nil
+  then show ?case by vcg
+next
+  case (Cons x xs')
+  note [vcg_rules] = Cons.IH
+  show ?case
+    apply (cases xsi; cases i; simp)
+    by vcg
+qed
+
+lemma oa_nth_rule[vcg_rules]:
+  \<open>llvm_htriple
+    (\<upharpoonleft>oa_assn xs ali ** \<upharpoonleft>snat.assn i ii ** \<up>\<^sub>d(i < length xs))
+    (oa_nth ali ii)
+    (\<lambda>x. \<upharpoonleft>oa_assn xs ali ** A (xs!i) x)\<close>
+  unfolding oa_nth_def oa_assn_def
+  by vcg
+
+lemma oa_hnr:
+  \<open>(uncurry oa_nth, uncurry (RETURN oo op_list_get))
+  \<in> [\<lambda>(xs, i). i < length xs]\<^sub>a oa_assn'\<^sup>k *\<^sub>a (snat_assn' TYPE(64))\<^sup>k \<rightarrow> A\<close>
+  unfolding op_list_get_def snat.assn_is_rel[symmetric] snat_rel_def
+  apply sepref_to_hoare
+  by vcg
+
+section \<open>Update\<close>
+
+text \<open>We reuse the existing @{term arl_upd} implementation and leave
+  copying to the caller.\<close>
+
+definition oa_upd :: \<open>('b, 64) array_list \<Rightarrow> 64 word \<Rightarrow> 'b \<Rightarrow> ('b, 64) array_list llM\<close>
+  where [llvm_code]:
+  \<open>oa_upd ai ii xi \<equiv> doM {
+    old \<leftarrow> arl_nth ai ii;
+    afree old;
+    arl_upd ai ii xi
+  }\<close>
+
+lemma list_assn_afree_set_rule[vcg_rules]:
+  \<open>llvm_htriple
+     (\<upharpoonleft>(list_assn (mk_assn A)) xs xsi ** A x xi ** \<up>\<^sub>d(i < length xs))
+     (afree (xsi!i))
+     (\<lambda>_. \<upharpoonleft>(list_assn (mk_assn A)) (xs[i:=x]) (xsi[i:=xi]))\<close>
+proof (induction xs arbitrary: i xsi)
+  case Nil
+  then show ?case by vcg
+next
+  case (Cons y ys)
+  note [vcg_rules] = Cons.IH
+  show ?case
+    apply (cases xsi; cases i; simp)
+    by vcg
+qed
+
+lemma oa_upd_rule[vcg_rules]:
+  \<open>llvm_htriple
+    (\<upharpoonleft>oa_assn xs ali ** \<upharpoonleft>snat.assn i ii ** A x xi ** \<up>\<^sub>d(i < length xs))
+    (oa_upd ali ii xi)
+    (\<lambda>r. \<up>(r = ali) ** \<upharpoonleft>oa_assn (xs[i:=x]) ali)\<close>
+  unfolding oa_upd_def oa_assn_def
+  by vcg
+
+lemma oa_upd_hnr:
+  \<open>(uncurry2 oa_upd, uncurry2 (RETURN ooo op_list_set))
+  \<in> [\<lambda>((xs, i), x). i < length xs]\<^sub>a oa_assn'\<^sup>d *\<^sub>a (snat_assn' TYPE(64))\<^sup>k *\<^sub>a A\<^sup>d \<rightarrow> oa_assn'\<close>
+  unfolding op_list_set_def snat_rel_def snat.assn_is_rel[symmetric]
+  apply sepref_to_hoare
+  by vcg
+
+section \<open>Push back\<close>
+
+definition oa_push_back :: \<open>('b, 64) array_list \<Rightarrow> 'b \<Rightarrow> ('b, 64) array_list llM\<close>
+  where [llvm_code, llvm_inline]:
+  \<open>oa_push_back ai xi \<equiv> arl_push_back ai xi\<close>
+
+lemma oa_push_back_aux:
+  \<open>ENTAILS
+     (\<upharpoonleft>arl_assn (xsi @ [xi]) ali \<and>* \<upharpoonleft>(list_assn (mk_assn A)) xs xsi \<and>* A x xi)
+     (\<lambda>c. \<exists>xsi'. (\<upharpoonleft>arl_assn xsi' ali \<and>* \<upharpoonleft>(list_assn (mk_assn A)) (xs @ [x]) xsi') c)\<close>
+  unfolding ENTAILS_def
+  apply (rule entails_pureI)
+  apply (clarsimp dest!: pure_part_split_conj list_assn_pure_part)
+  apply (rule entails_exI[where x=\<open>xsi @ [xi]\<close>])
+  by (simp add: sep_algebra_simps sep_conj_aci)
+
+lemma oa_push_back_rule[vcg_rules]:
+  \<open>llvm_htriple
+    (\<upharpoonleft>oa_assn xs ali ** A x xi ** \<up>\<^sub>d(length xs + 1 < max_snat 64))
+    (oa_push_back ali xi)
+    (\<lambda>ali'. \<upharpoonleft>oa_assn (xs @ [x]) ali')\<close>
+  unfolding oa_push_back_def oa_assn_def
+  apply vcg
+  by (rule oa_push_back_aux)
+
+lemma oa_push_back_hnr:
+  \<open>(uncurry oa_push_back, uncurry (RETURN oo op_list_append))
+  \<in> [\<lambda>(xs, _). length xs + 1 < max_snat 64]\<^sub>a oa_assn'\<^sup>d *\<^sub>a A\<^sup>d \<rightarrow> oa_assn'\<close>
+  unfolding op_list_append_def
+  apply sepref_to_hoare
+  by vcg
+
+section \<open>Length\<close>
+
+definition oa_len :: \<open>('b, 64) array_list \<Rightarrow> 64 word llM\<close> where [llvm_code, llvm_inline]:
+  \<open>oa_len ai \<equiv> arl_len ai\<close>
+
+lemma oa_len_aux:
+  assumes L: \<open>\<flat>\<^sub>psnat.assn (length xsi) li\<close>
+  shows \<open>ENTAILS
+     (\<upharpoonleft>arl_assn xsi ali \<and>* \<upharpoonleft>(list_assn (mk_assn A)) xs xsi)
+     ((\<lambda>a. \<exists>xsi'. (\<upharpoonleft>arl_assn xsi' ali \<and>* \<upharpoonleft>(list_assn (mk_assn A)) xs xsi') a)
+       \<and>* \<upharpoonleft>snat.assn (length xs) li)\<close>
+  unfolding ENTAILS_def
+  apply (rule entails_pureI)
+  apply (clarsimp dest!: pure_part_split_conj list_assn_pure_part)
+  apply (simp add: snat.assn_pure[THEN extract_pure_assn] L sep_algebra_simps
+    pred_lift_extract_simps)
+  apply (rule entails_exI[where x=xsi])
+  by (rule entails_refl)
+
+lemma oa_len_rule[vcg_rules]:
+  \<open>llvm_htriple (\<upharpoonleft>oa_assn xs ali) (oa_len ali)
+    (\<lambda>li. \<upharpoonleft>oa_assn xs ali ** \<upharpoonleft>snat.assn (length xs) li)\<close>
+  unfolding oa_len_def oa_assn_def
+  apply vcg
+  by (rule oa_len_aux)
+
+lemma oa_len_hnr:
+  \<open>(oa_len, RETURN o op_list_length) \<in> oa_assn'\<^sup>k \<rightarrow>\<^sub>a snat_assn' TYPE(64)\<close>
+  unfolding op_list_length_def snat_rel_def snat.assn_is_rel[symmetric]
+  apply sepref_to_hoare
+  by vcg
+
+section \<open>Empty\<close>
+
+lemma oa_empty_rule[vcg_rules]:
+  \<open>llvm_htriple \<box> (arl_new TYPE('b) TYPE(64)) (\<lambda>ali. \<upharpoonleft>oa_assn [] ali)\<close>
+  unfolding oa_assn_def
+  by vcg
+
+definition oa_empty :: \<open>('b, 64) array_list llM\<close> where [llvm_code, llvm_inline]:
+  \<open>oa_empty \<equiv> arl_new TYPE('b) TYPE(64)\<close>
+
+lemma oa_empty_hnr:
+  \<open>(uncurry0 oa_empty, uncurry0 (RETURN op_list_empty)) \<in> unit_assn\<^sup>k \<rightarrow>\<^sub>a oa_assn'\<close>
+  unfolding oa_empty_def op_list_empty_def
+  apply sepref_to_hoare
+  by vcg
+
+section \<open>Free\<close>
+text \<open>We need to also free the inner elements.\<close>
+
+definition oa_free :: \<open>('b, 64) array_list \<Rightarrow> unit llM\<close> where [llvm_code]:
+  \<open>oa_free ai \<equiv> doM {
+  llc_while
+    (\<lambda>i. doM{ l \<leftarrow> oa_len ai; ll_icmp_ult i l })
+    (\<lambda>i. doM {
+      xi \<leftarrow> arl_nth ai i;
+      afree xi;
+      i \<leftarrow> ll_add i (signed_nat 1);
+      Mreturn i
+    }) (signed_nat 0);
+    arl_free ai
+  }\<close>
+
+lemma oa_free_aux_rule:
+  \<open>llvm_htriple
+    (\<upharpoonleft>arl_assn xsi ali ** \<upharpoonleft>(list_assn (mk_assn A)) xs xsi)
+    (oa_free ali)
+    (\<lambda>_. \<box>)\<close>
+  unfolding oa_free_def oa_len_def
+  apply (rewrite annotate_llc_while[where
+    I=\<open>\<lambda>ii t. EXS i. \<upharpoonleft>snat.assn i ii ** \<upharpoonleft>arl_assn xsi ali
+        ** \<upharpoonleft>(list_assn (mk_assn A)) (drop i xs) (drop i xsi)
+        ** \<up>\<^sub>!(i \<le> length xs \<and> length xsi = length xs \<and> t = length xs - i)\<close>
+    and R=\<open>less_than\<close>])
+  supply [simp] = Cons_nth_drop_Suc[symmetric]
+  apply vcg_monadify
+  apply vcg'
+  done
+
+lemma oa_free_rule[vcg_rules]:
+  \<open>llvm_htriple (\<upharpoonleft>oa_assn xs ali) (oa_free ali) (\<lambda>_. \<box>)\<close>
+  unfolding oa_assn_def
+  supply [vcg_rules] = oa_free_aux_rule
+  by vcg
+
+lemma oa_free_mk_free[sepref_frame_free_rules]: \<open>MK_FREE oa_assn' oa_free\<close>
+  by (rule MK_FREEI) (rule oa_free_rule)
+
+end
+
+section \<open>Instantiation for string tables\<close>
+
+interpretation strls: copyable_assn strl_assn' strl.cl_free strl.cl_copy
+  apply unfold_locales
+  subgoal by (rule strl.cl_assn_free)
+  subgoal by (rule strl.cl_copy_hnr)
+  done
+
+abbreviation \<open>strls_assn \<equiv> \<upharpoonleft>strls.oa_assn\<close>
+
+end
